$2_{x}$ 

$x^{2}$ + 2 = $e^{-alpha t}$

$a^{3}_{ij}$

$e^{x^2}$

$\sqrt{x}$

$\sqrt{x^{2} + \sqrt{y} }$ 

 $\surd[x^2 + y^2]$

$\overline{m+n}$

$\underline{m+n}$

$\underbrace{a+b+\cdots+z}_{26}$

$x^\prime$

$\vec{c}$

$\overrightarrow{c d}$

$\sum_{k=1}^N k^2$

$\lim_{n \to 0}x_n$

$\lim_{n \to \infty}x_n$

$\frac{2}{4}$

$\cfrac{2}{5 + \cfrac{2}{d + \cfrac{1}{\lim_{n \to 0}x_n}}}$

$C^n_r$

$\begin{cases}
3x + 5y + z \

7x - 2y + 4z \

-6x + 3y +2z
\end{cases}$

$\in$

$\sqrt{n}{3}$

$\because$

$\therefore$

例子：打出一个证明题

$\because$ Position Notation $(x)_{2}$ = $\sum_{i=1}^k d_{i}2^{i-1}$

$\because$ Two's complement

N(x) = $2^{k}$ - x , where k is the number of bits for an integer

and , $N^\prime(x)$ = $\2^{m}$ - x where m > k

$\therefore$ $N^\prime(x)$ = $2^{m}$ - x = ($2^{m}$ - $2^{k}$ ) + $2^{k}$ - x = ($2^{m}$ - 1) - ($2^{k}$ - 1) + N(x)

$\because$ $2^{m} - 1 = (2-1)\sum_{i=1}^m 2^{i-1}$ , that